examples/sbf/verif_Filter_query.v
@@ -1,0 +1,502 @@
+Require Import Poulet4.P4light.Syntax.P4defs.
+Require Import Poulet4.P4light.Semantics.Semantics.
+Require Import ProD3.core.Core.
+Require Import ProD3.core.Tofino.
+Require Import ProD3.examples.sbf.p4ast.
+Require Import ProD3.examples.sbf.ConFilter.
+Require Import ProD3.examples.sbf.common.
+Require Import ProD3.examples.sbf.FilterRepr.
+Require Import ProD3.examples.sbf.verif_Win1.
+Require Import ProD3.examples.sbf.verif_Win2.
+Require Import ProD3.examples.sbf.verif_Win3.
+Require Import ProD3.examples.sbf.verif_Win4.
+Require Import ProD3.examples.sbf.verif_Filter.
+
+#[local] Hint Extern 5 (func_modifies _ _ _ _ _) => (apply tbl_hash_index_1_body) : func_specs.
+#[local] Hint Extern 5 (func_modifies _ _ _ _ _) => (apply tbl_hash_index_1_body) : func_specs.
+#[local] Hint Extern 5 (func_modifies _ _ _ _ _) => (apply tbl_hash_index_1_body) : func_specs.
+#[local] Hint Extern 5 (func_modifies _ _ _ _ _) => (apply tbl_clear_index_body) : func_specs.
+#[local] Hint Extern 5 (func_modifies _ _ _ _ _) => (apply tbl_clear_window_body) : func_specs.
+#[local] Hint Extern 5 (func_modifies _ _ _ _ _) => (apply act_set_clear_win_1_body) : func_specs.
+#[local] Hint Extern 5 (func_modifies _ _ _ _ _) => (apply act_set_clear_win_2_body) : func_specs.
+#[local] Hint Extern 5 (func_modifies _ _ _ _ _) => (apply act_set_clear_win_3_body) : func_specs.
+#[local] Hint Extern 5 (func_modifies _ _ _ _ _) => (apply act_set_clear_win_4_body) : func_specs.
+
+Definition P4_bf2_win_md_t_query (f cf if' : Z) (new_clear_index : Sval) (is : list Sval) :=
+  if f=? cf then
+    P4_bf2_win_md_t (P4Bit 8 CLEAR) (Zrepeat new_clear_index 3)
+  else
+    P4_bf2_win_md_t (P4Bit 8 QUERY) is.
+
+Definition tbl_set_win_query_spec : func_spec :=
+  WITH (* p *),
+    PATH p
+    MOD (Some [["ds_md"];
+               ["act_set_clear_win_1"; "api_1"];
+               ["act_set_clear_win_1"; "api_2"];
+               ["act_set_clear_win_1"; "api_3"];
+               ["act_set_clear_win_1"; "api_4"];
+               ["act_set_clear_win_2"; "api_1"];
+               ["act_set_clear_win_2"; "api_2"];
+               ["act_set_clear_win_2"; "api_3"];
+               ["act_set_clear_win_2"; "api_4"];
+               ["act_set_clear_win_3"; "api_1"];
+               ["act_set_clear_win_3"; "api_2"];
+               ["act_set_clear_win_3"; "api_3"];
+               ["act_set_clear_win_3"; "api_4"];
+               ["act_set_clear_win_2"; "api_1"];
+               ["act_set_clear_win_4"; "api_1"];
+               ["act_set_clear_win_4"; "api_2"];
+               ["act_set_clear_win_4"; "api_3"];
+               ["act_set_clear_win_4"; "api_4"]]) []
+    WITH (timer : Z * bool) (clear_index_1 hash_index_1 hash_index_2 hash_index_3: Sval)
+      (H_timer : 0 <= fst timer < frame_tick_tocks * num_frames),
+      PRE
+        (ARG []
+        (MEM [(["api"], P4Bit 8 QUERY);
+              (["ds_md"], ValBaseStruct
+                 [("clear_window", P4Bit 16 (fst timer));
+                  ("clear_index_1", clear_index_1);
+                  ("hash_index_1", hash_index_1);
+                  ("hash_index_2", hash_index_2);
+                  ("hash_index_3", hash_index_3);
+                  ("win_1", P4_bf2_win_md_t_);
+                  ("win_2", P4_bf2_win_md_t_);
+                  ("win_3", P4_bf2_win_md_t_);
+                  ("win_4", P4_bf2_win_md_t_)])]
+        (EXT [])))
+      POST
+        (EX retv,
+        (ARG_RET [] retv
+        (let cf := get_clear_frame timer in
+        let if' := get_insert_frame cf in
+        (MEM [(["ds_md"], ValBaseStruct
+                 [("clear_window", P4Bit 16 (fst timer));
+                  ("clear_index_1", clear_index_1);
+                  ("hash_index_1", hash_index_1);
+                  ("hash_index_2", hash_index_2);
+                  ("hash_index_3", hash_index_3);
+                  ("win_1", P4_bf2_win_md_t_query 0 cf if' clear_index_1
+                        [hash_index_1; hash_index_2; hash_index_3]);
+                  ("win_2", P4_bf2_win_md_t_query 1 cf if' clear_index_1
+                        [hash_index_1; hash_index_2; hash_index_3]);
+                  ("win_3", P4_bf2_win_md_t_query 2 cf if' clear_index_1
+                        [hash_index_1; hash_index_2; hash_index_3]);
+                  ("win_4", P4_bf2_win_md_t_query 3 cf if' clear_index_1
+                        [hash_index_1; hash_index_2; hash_index_3])])]
+        (EXT [])))))%arg_ret_assr.
+
+Lemma tbl_set_win_query_body :
+  func_sound ge tbl_set_win_fd nil tbl_set_win_query_spec.
+Admitted.
+
+Definition act_merge_wins_fd :=
+  ltac:(get_fd ["Bf2BloomFilter"; "act_merge_wins"] ge).
+
+Definition act_merge_wins_spec : func_spec :=
+  WITH (* p *),
+    PATH p
+    MOD (Some [["query_res"]]) []
+    WITH,
+      PRE
+        (ARG []
+        (MEM []
+        (EXT [])))
+      POST
+        (ARG_RET [] ValBaseNull
+        (MEM [(["query_res"], (P4Bit 8 1))]
+        (EXT []))).
+
+Lemma act_merge_wins_body :
+  func_sound ge act_merge_wins_fd nil act_merge_wins_spec.
+Proof.
+  start_function.
+  step.
+  step.
+  entailer.
+Qed.
+
+Definition act_merge_default_fd :=
+  ltac:(get_fd ["Bf2BloomFilter"; "act_merge_default"] ge).
+
+Definition act_merge_default_spec : func_spec :=
+  WITH (* p *),
+    PATH p
+    MOD (Some [["query_res"]]) []
+    WITH,
+      PRE
+        (ARG []
+        (MEM []
+        (EXT [])))
+      POST
+        (ARG_RET [] ValBaseNull
+        (MEM [(["query_res"], (P4Bit 8 0))]
+        (EXT []))).
+
+Lemma act_merge_default_body :
+  func_sound ge act_merge_default_fd nil act_merge_default_spec.
+Proof.
+  start_function.
+  step.
+  step.
+  entailer.
+Qed.
+
+Definition tbl_merge_wins_fd :=
+  ltac:(get_fd ["Bf2BloomFilter"; "tbl_merge_wins"; "apply"] ge).
+
+Definition P4_bf2_win_md_t_rw rw1 rw2 rw3 :=
+  ValBaseStruct
+    [("api", P4Bit_ 8);
+     ("index_1", P4Bit_ 18);
+     ("index_2", P4Bit_ 18);
+     ("index_3", P4Bit_ 18);
+     ("rw_1", P4Bit 8 (Z.b2z rw1));
+     ("rw_2", P4Bit 8 (Z.b2z rw2));
+     ("rw_3", P4Bit 8 (Z.b2z rw3))].
+
+(* Because this function doesn't modify ds_md, so we can describe it in this way.
+But if it does modify ds_md, we don't have a really good way to isolate the unchanged part.
+But on the other hand, the get/update system doesn't work very well, either. *)
+Definition tbl_merge_wins_spec : func_spec :=
+  WITH (* p *),
+    PATH p
+    MOD (Some [["query_res"]]) []
+    WITH rw11 rw12 rw13 rw21 rw22 rw23 rw31 rw32 rw33 rw41 rw42 rw43,
+      PRE
+        (ARG []
+        (MEM [(["api"], P4Bit 8 QUERY);
+              (["ds_md"], ValBaseStruct
+                 [("clear_window", P4Bit_ 16);
+                  ("clear_index_1", P4Bit_ 18);
+                  ("hash_index_1", P4Bit_ 18);
+                  ("hash_index_2", P4Bit_ 18);
+                  ("hash_index_3", P4Bit_ 18);
+                  ("win_1", P4_bf2_win_md_t_rw rw11 rw12 rw13);
+                  ("win_2", P4_bf2_win_md_t_rw rw21 rw22 rw23);
+                  ("win_3", P4_bf2_win_md_t_rw rw31 rw32 rw33);
+                  ("win_4", P4_bf2_win_md_t_rw rw41 rw42 rw43)])]
+        (EXT [])))
+      POST
+        (EX retv,
+        (ARG_RET [] retv
+        (MEM [(["query_res"], (P4Bit 8 (Z.b2z (
+          fold_orb (map fold_andb
+            [[rw11; rw12; rw13];
+             [rw21; rw22; rw23];
+             [rw31; rw32; rw33];
+             [rw41; rw42; rw43]])))))]
+        (EXT []))))%arg_ret_assr.
+
+Lemma b2z_one : forall b,
+  Z.b2z b =? 1 = b.
+Proof.
+  destruct b; auto.
+Qed.
+
+Lemma tbl_merge_wins_body :
+  func_sound ge tbl_merge_wins_fd nil tbl_merge_wins_spec.
+Proof.
+  start_function.
+  unfold P4_bf2_win_md_t_rw.
+  hoare_table_action_cases';
+    repeat rewrite b2z_one in *;
+    repeat lazymatch goal with
+    | H : is_true (_ && _) |- _ =>
+        apply Reflect.andE in H;
+        destruct H
+    end;
+    repeat match goal with
+    | H : is_true ?b |- _ =>
+        is_var b;
+        unfold is_true in H;
+        subst b
+    end.
+  - table_action act_merge_wins_body.
+    { entailer. }
+    { entailer. }
+
+#[export] Hint Rewrite Bool.orb_true_l Bool.orb_true_r Bool.orb_false_l Bool.orb_false_r : simpl_orb.
+
+  - table_action act_merge_wins_body.
+    { entailer. }
+    { entailer.
+      unfold map, fold_andb, fold_orb, fold_left.
+      autorewrite with simpl_andb simpl_orb.
+      apply sval_refine_refl.
+    }
+  - table_action act_merge_wins_body.
+    { entailer. }
+    { entailer.
+      unfold map, fold_andb, fold_orb, fold_left.
+      autorewrite with simpl_andb simpl_orb.
+      apply sval_refine_refl.
+    }
+  - table_action act_merge_wins_body.
+    { entailer. }
+    { entailer.
+      unfold map, fold_andb, fold_orb, fold_left.
+      autorewrite with simpl_andb simpl_orb.
+      apply sval_refine_refl.
+    }
+  - table_action act_merge_default_body.
+    { entailer. }
+    { entailer.
+      unfold map, fold_andb, fold_orb, fold_left.
+      autorewrite with simpl_andb simpl_orb.
+      replace (rw11 && rw12 && rw13) with false by (destruct (rw11 && rw12 && rw13); auto).
+      replace (rw21 && rw22 && rw23) with false by (destruct (rw21 && rw22 && rw23); auto).
+      replace (rw31 && rw32 && rw33) with false by (destruct (rw31 && rw32 && rw33); auto).
+      replace (rw41 && rw42 && rw43) with false by (destruct (rw41 && rw42 && rw43); auto).
+      apply sval_refine_refl.
+    }
+  - elim_trivial_cases.
+  - elim_trivial_cases.
+Qed.
+
+Definition filter_query := @filter_query num_frames num_rows num_slots ltac:(lia) ltac:(lia) ltac:(lia)
+  frame_tick_tocks.
+
+Definition Filter_query_spec : func_spec :=
+  WITH (* p *),
+    PATH p
+    MOD None [p]
+    WITH (key : Val) (tstamp : Z) (cf : filter num_frames num_rows num_slots),
+      PRE
+        (ARG [eval_val_to_sval key; P4Bit 8 QUERY; P4Bit 48 tstamp; P4Bit_ 8]
+        (MEM []
+        (EXT [filter_repr p 18 panes rows cf])))
+      POST
+        (ARG_RET [P4Bit 8 (Z.b2z (snd (filter_query cf (Z.odd (tstamp/2097152)) (hashes key))))] ValBaseNull
+        (MEM []
+        (EXT [filter_repr p 18 panes rows (fst (filter_query cf (Z.odd (tstamp/2097152)) (hashes key)))]))).
+
+Ltac destruct_listn l :=
+  destruct l as [l ?H];
+  destruct_list l.
+
+Lemma Filter_query_body :
+  func_sound ge Filter_fd nil Filter_query_spec.
+Proof.
+  start_function.
+  destruct cf as [[ps ?H] ? ?].
+  unfold filter_repr.
+  cbn [proj1_sig] in *.
+  destruct_list ps.
+  normalize_EXT.
+  step.
+  step_call tbl_hash_index_1_body.
+  { entailer. }
+  Intros _.
+  step_call tbl_hash_index_2_body.
+  { entailer. }
+  Intros _.
+  step_call tbl_hash_index_3_body.
+  { entailer. }
+  Intros _.
+  set (is := (exist _ [hash1 key; hash2 key; hash3 key] eq_refl : listn Z 3)).
+  set (clear_is := (exist _ (Zrepeat fil_clear_index 3) eq_refl : listn Z 3)).
+  assert (Forall (fun i : Z => 0 <= i < num_slots) (`is)). {
+    repeat first [apply Forall_cons | apply Forall_nil].
+    all : unfold hash1, hash2, hash3;
+      apply Z.mod_pos_bound; lia.
+  }
+  P4assert (0 <= fil_clear_index < num_slots). {
+    unfold fil_clear_index_repr.
+    Intros i'.
+    normalize_EXT.
+    Intros_prop.
+    apply ext_implies_prop_intro.
+    subst.
+    apply Z.mod_pos_bound.
+    lia.
+  }
+  assert (Forall (fun i : Z => 0 <= i < num_slots) (`clear_is)). {
+    repeat first [
+      assumption
+    | constructor
+    ].
+  }
+  step_call tbl_clear_index_body.
+  { entailer. }
+  Intros _.
+  step_call tbl_clear_window_body.
+  { entailer. }
+  Intros _.
+  set (new_timer := update_timer fil_timer (Z.odd (tstamp / 2097152))).
+  P4assert (0 <= fst new_timer < num_frames * frame_tick_tocks).
+  { unfold timer_repr.
+    normalize_EXT.
+    Intros_prop.
+    apply ext_implies_prop_intro.
+    auto.
+  }
+  step_call tbl_set_win_query_body.
+  { entailer. }
+  { auto. }
+  Intros _.
+  (* unfold and fold in the post condition *)
+  unfold filter_query, ConFilter.filter_query.
+  (* cbn [proj1_sig fst snd]. *)
+  unfold proj1_sig. unfold fst. unfold snd.
+  fold new_timer.
+  replace (exist (fun i : list Z => Zlength i = num_rows) (Zrepeat fil_clear_index num_rows) _) with clear_is. 2 : {
+    apply subset_eq_compat. auto.
+  }
+  assert (0 <= get_clear_frame new_timer < num_frames). {
+    unfold ConFilter.get_clear_frame.
+    split.
+    - apply Z.div_le_lower_bound; lia.
+    - apply Z.div_lt_upper_bound; lia.
+  }
+  destruct (get_clear_frame new_timer =? 0) eqn:?.
+  { replace (get_clear_frame new_timer) with 0 by lia.
+    step_call verif_Win1.Win_body _ _ clear_is.
+    { entailer. }
+    { solve [repeat constructor]. }
+    { auto. }
+    step_call verif_Win2.Win_body _ _ is.
+    { entailer. }
+    { solve [repeat constructor]. }
+    { auto. }
+    step_call verif_Win3.Win_body _ _ is.
+    { entailer. }
+    { solve [repeat constructor]. }
+    { auto. }
+    step_call verif_Win4.Win_body _ _ is.
+    { entailer. }
+    { solve [repeat constructor]. }
+    { auto. }
+    simpl Z.eqb. cbn match.
+    step_call tbl_merge_wins_body.
+    { unfold P4_bf2_win_md_t_rw.
+      entailer.
+      replace (P4Bit 8 0) with (P4Bit 8 (Z.b2z false)) by auto.
+      repeat first [
+        apply sval_refine_refl
+      | constructor
+      ].
+    }
+    Intros _.
+    step.
+    entailer.
+    destruct_listn x.
+    destruct_listn x0.
+    destruct_listn x1.
+    destruct_listn x2.
+    apply sval_refine_refl.
+  }
+  destruct (get_clear_frame new_timer =? 1) eqn:?.
+  { replace (get_clear_frame new_timer) with 1 by lia.
+    step_call verif_Win1.Win_body _ _ is.
+    { entailer. }
+    { solve [repeat constructor]. }
+    { auto. }
+    step_call verif_Win2.Win_body _ _ clear_is.
+    { entailer. }
+    { solve [repeat constructor]. }
+    { auto. }
+    step_call verif_Win3.Win_body _ _ is.
+    { entailer. }
+    { solve [repeat constructor]. }
+    { auto. }
+    step_call verif_Win4.Win_body _ _ is.
+    { entailer. }
+    { solve [repeat constructor]. }
+    { auto. }
+    simpl Z.eqb. cbn match.
+    step_call tbl_merge_wins_body.
+    { unfold P4_bf2_win_md_t_rw.
+      entailer.
+      replace (P4Bit 8 0) with (P4Bit 8 (Z.b2z false)) by auto.
+      repeat first [
+        apply sval_refine_refl
+      | constructor
+      ].
+    }
+    Intros _.
+    step.
+    entailer.
+    destruct_listn x.
+    destruct_listn x0.
+    destruct_listn x1.
+    destruct_listn x2.
+    apply sval_refine_refl.
+  }
+  destruct (get_clear_frame new_timer =? 2) eqn:?.
+  { replace (get_clear_frame new_timer) with 2 by lia.
+    step_call verif_Win1.Win_body _ _ is.
+    { entailer. }
+    { solve [repeat constructor]. }
+    { auto. }
+    step_call verif_Win2.Win_body _ _ is.
+    { entailer. }
+    { solve [repeat constructor]. }
+    { auto. }
+    step_call verif_Win3.Win_body _ _ clear_is.
+    { entailer. }
+    { solve [repeat constructor]. }
+    { auto. }
+    step_call verif_Win4.Win_body _ _ is.
+    { entailer. }
+    { solve [repeat constructor]. }
+    { auto. }
+    simpl Z.eqb. cbn match.
+    step_call tbl_merge_wins_body.
+    { unfold P4_bf2_win_md_t_rw.
+      entailer.
+      replace (P4Bit 8 0) with (P4Bit 8 (Z.b2z false)) by auto.
+      repeat first [
+        apply sval_refine_refl
+      | constructor
+      ].
+    }
+    Intros _.
+    step.
+    entailer.
+    destruct_listn x.
+    destruct_listn x0.
+    destruct_listn x1.
+    destruct_listn x2.
+    apply sval_refine_refl.
+  }
+  destruct (get_clear_frame new_timer =? 3) eqn:?.
+  { replace (get_clear_frame new_timer) with 3 by lia.
+    step_call verif_Win1.Win_body _ _ is.
+    { entailer. }
+    { solve [repeat constructor]. }
+    { auto. }
+    step_call verif_Win2.Win_body _ _ is.
+    { entailer. }
+    { solve [repeat constructor]. }
+    { auto. }
+    step_call verif_Win3.Win_body _ _ is.
+    { entailer. }
+    { solve [repeat constructor]. }
+    { auto. }
+    step_call verif_Win4.Win_body _ _ clear_is.
+    { entailer. }
+    { solve [repeat constructor]. }
+    { auto. }
+    simpl Z.eqb. cbn match.
+    step_call tbl_merge_wins_body.
+    { unfold P4_bf2_win_md_t_rw.
+      entailer.
+      replace (P4Bit 8 0) with (P4Bit 8 (Z.b2z false)) by auto.
+      repeat first [
+        apply sval_refine_refl
+      | constructor
+      ].
+    }
+    Intros _.
+    step.
+    entailer.
+    destruct_listn x.
+    destruct_listn x0.
+    destruct_listn x1.
+    destruct_listn x2.
+    apply sval_refine_refl.
+  }
+  lia.
+(* This is slow. I can understand it but I don't know the direct reason. *)
+Time Qed.
